silveroak-opentitan/aes/Acorn/CipherControlNetlist.v
@@ -34,6 +34,37 @@ Import Pkg.Notations.
 
 Require Import AcornAes.ShiftRowsNetlist.
 Require Import AcornAes.MixColumnsNetlist.
+Require Import AcornAes.SubBytesNetlist.
+
+Definition aes_shift_rows' x y :=
+  blackBoxNet aes_shift_rows_Interface (x, y).
+Definition aes_mix_columns' x y :=
+  blackBoxNet aes_mix_columns_Interface (x, y).
+Definition aes_sbox_lut' x y :=
+  blackBoxNet aes_sbox_lut_Interface (x, y).
+Definition aes_sub_bytes' (is_decrypt : Signal Bit) (b : Signal state)
+  : cava (Signal state) := state_map (aes_sbox_lut' is_decrypt) b.
+
+Definition inv_mix_columns_key := aes_mix_columns' (constant true).
+
+(* Interface of existing aes_key_expand
+* https://github.com/lowRISC/opentitan/blob/783edaf444eb0d9eaf9df71c785089bffcda574e/hw/ip/aes/rtl/aes_key_expand.sv *)
+Definition aes_key_expand_Interface :=
+   sequentialInterface "aes_key_expand"
+   "clk_i" PositiveEdge "rst_ni" NegativeEdge
+   [ mkPort "op_i" Bit
+   ; mkPort "step_i" Bit
+   ; mkPort "clear_i" Bit
+   ; mkPort "round_i" (Vec Bit 4)
+   ; mkPort "key_len_i" (Vec Bit 3)
+   ; mkPort "key_i" key
+   ]
+   [ mkPort "key_o" key ]
+   [].
+
+Definition aes_key_expand :
+  Circuit _ _ :=
+  Comb (blackBoxNet aes_key_expand_Interface).
 
 Definition cipher_round := CipherCircuit.cipher_round
   (round_index:=round_index)
@@ -54,4 +85,41 @@ Definition cipher_round_Interface :=
 Definition cipher_round_Netlist
   := makeNetlist cipher_round_Interface
   (fun '(a, b, c, d, e, f ) => cipher_round a b c d e f).
+
+Definition aes_cipher_core_Interface :=
+  sequentialInterface "aes_cipher_core"
+  "clk_i" PositiveEdge
+  "rst_ni" NegativeEdge
+  [ mkPort "in_valid_i" Bit
+  ; mkPort "out_ready_i" Bit
+  ; mkPort "crypt_i" Bit
+  ; mkPort "dec_key_gen_i" Bit
+  ; mkPort "key_clear_i" Bit
+  ; mkPort "data_out_clear_i" Bit
+  ; mkPort "op_i" Bit
+  ; mkPort "key_len_i" (Vec Bit 3)
+
+  ; mkPort "prng_data_i" state
+  ; mkPort "state_init_i" state
+  ; mkPort "key_init_i" key
+
+  ]
+  [ mkPort "in_ready_o" Bit
+  ; mkPort "out_valid_o" Bit
+  ; mkPort "crypt_o" Bit
+  ; mkPort "dec_key_gen_o" Bit
+  ; mkPort "key_clear_o" Bit
+  ; mkPort "state_o" state
+  ]
+  [].
+
+Definition cipher_loop := CipherCircuit.cipher_loop
+  (round_index:=round_index)
+  aes_sub_bytes' aes_shift_rows' aes_mix_columns' aes_add_round_key
+  inv_mix_columns_key.
+Definition aes_cipher_core := CipherControlCircuit.aes_cipher_core
+  aes_key_expand cipher_loop.
+
+Definition aes_cipher_core_Netlist
+  := makeCircuitNetlist aes_cipher_core_Interface aes_cipher_core.
 
